src/ecEnv.ml
@@ -172,7 +172,7 @@ type crb_tyrev_binding = [
   | `Array     of crb_array
 ]
 
-type crb_bitstring_operator = crb_bitstring * [`From | `To | `OfInt | `ToInt]
+type crb_bitstring_operator = crb_bitstring * [`From | `To | `OfInt | `ToUInt | `ToSInt ]
 
 type crb_array_operator = crb_array * [`Get | `Set | `ToList | `OfList]
 
@@ -2862,7 +2862,8 @@ module Circuit = struct
             bindings.opreverse
             [ (bs.from_, `Bitstring (bs, `From ))
             ; (bs.to_  , `Bitstring (bs, `To   ))
-            ; (bs.toint, `Bitstring (bs, `ToInt))
+            ; (bs.touint, `Bitstring (bs, `ToUInt))
+            ; (bs.tosint, `Bitstring (bs, `ToSInt))
             ; (bs.ofint, `Bitstring (bs, `OfInt)) ]; }
 
   let rebind_bitstring (bs : crb_bitstring) (env : env) : env =
