src/ecSubst.ml
@@ -1041,13 +1041,15 @@ let subst_crbinding (s : subst) (crb : crbinding) =
     assert (not (Mp.mem bs.type_ s.sb_tydef));
     assert (not (Mp.mem bs.from_ s.sb_def));
     assert (not (Mp.mem bs.to_ s.sb_def));
-    assert (not (Mp.mem bs.toint s.sb_def));
+    assert (not (Mp.mem bs.touint s.sb_def));
+    assert (not (Mp.mem bs.tosint s.sb_def));
     assert (not (Mp.mem bs.ofint s.sb_def));
     CRB_Bitstring {
       type_  = subst_path s bs.type_;
       from_  = subst_path s bs.from_;
       to_    = subst_path s bs.to_;
-      toint  = subst_path s bs.toint;
+      touint  = subst_path s bs.touint;
+      tosint  = subst_path s bs.tosint;
       ofint  = subst_path s bs.ofint;
       size   = bs.size;
       theory = subst_path s bs.theory; }
